project2/grep-naive/grep.dfy
@@ -8,14 +8,24 @@
 include "Io.dfy"
 include "FileUtils.dfy"
 
-function method match_at(t: seq<byte>, p:seq<byte>, t_pos:nat): bool
-    requires 0 <= t_pos < |t|
+predicate method match_at<T(==)>(t: seq<T>, p:seq<T>, pos:nat)
+    requires 0 <= pos < |t|
 {
-    p <= t[t_pos..]
+    pos + |p| <= |t| && p == t[pos..pos+|p|]
 }
+
+predicate any_match<T(==)>(t: seq<T>, p:seq<T>, pos:nat)
+  decreases t
+  requires 0 <= pos <= |t|
+{
+  exists i :: 0 <= i < pos && match_at(t, p, i)
+}
+
 
 method first_match(t: seq<byte>, p:seq<byte>) returns (found: bool, s:nat)
   requires |t| != 0
+
+  ensures any_match(t, p, |t|) <==> found
   ensures found ==> 0 <= s < |t|
   ensures !found ==> 0 <= s <= |t|
   ensures found ==> match_at(t, p, s)
@@ -23,45 +33,50 @@ method first_match(t: seq<byte>, p:seq<byte>) returns (found: bool, s:nat)
 {
   s := 0;
   found := false;
-  while s < |t| - |p|
+  while s < |t|
     decreases |t| - s
     invariant s <= |t|
     invariant forall k :: 0 <= k < s ==> !match_at(t, p, k)
+    invariant !any_match(t, p, s)
   {
     if match_at(t, p, s) {
       found := true;
       return;
     }
+
     s := s + 1;
   }
 }
 
-method Grep(file: FileStream, length: int32, pattern: seq<byte>)
+method Grep(file: FileStream, length: int32, pattern: seq<byte>) returns (ok:bool, found: bool, s:nat)
   requires FileOk(file)
   requires length as int == len(file)
 
   modifies file
   modifies file.env.ok
   modifies file.env.files
+
+  ensures ok ==> FileOk(file)
+  ensures ok ==> found ==> 0 <= s < |content(file)|
+  ensures ok ==> !found ==> 0 <= s <= |content(file)|
+  ensures ok ==> found ==> match_at(content(file), pattern, s)
+  ensures ok ==> forall k :: 0 <= k < s ==> !match_at(content(file), pattern, k)
 {
-  var ok, cont := ReadFile(file, length as nat32);
+  var cont;
+  ok, cont := ReadFile(file, length as nat32);
   if (!ok) {
     return;
   }
 
   if (|cont| == 0) {
     print "NO\n";
+    found := false;
+    s := 0;
     return;
   }
 
-  var m, n := first_match(cont, pattern);
-  if (m) {
-    print "YES: ";
-    print n;
-    print "\n";
-  } else {
-    print "NO\n";
-  }
+  found, s := first_match(cont, pattern);
+  
 }
 
 method {:main} Main(ghost env:HostEnvironment?)
@@ -97,10 +112,11 @@ method {:main} Main(ghost env:HostEnvironment?)
     return;
   }
 
-  Grep(src_file, src_len, seqa2seqb(pattern[..]));
+  var ok, m, n := Grep(src_file, src_len, seqa2seqb(pattern[..]));
 }
 
 function method {:verify false} seqa2seqb(s: seq<char>): seq<byte>
+  decreases s
 {
   if s == [] then [] else [s[0] as byte] + seqa2seqb(s[1..])
 }
