project2/grep-kmp/FileUtils.dfy
@@ -58,3 +58,22 @@ method ReadFile(f: FileStream, length: nat32) returns (ok: bool, result: seq<byt
 
     result := buffer[..];
 }
+
+method WriteFile(f: FileStream, s: seq<byte>) returns (ok: bool)
+    requires FileOk(f)
+    requires -0x80000000 <= |s| < 0x80000000
+    requires len(f) == 0
+
+    modifies f
+    modifies f.env.ok
+    modifies f.env.files
+
+    ensures ok ==> FileOk(f)
+    ensures ok ==> len(f) == |s|
+{
+    var buffer := ArrayFromSeq(s);
+    ok := f.Write(0, buffer, 0, |s| as int32);
+    if (!ok) {
+        return;
+    }
+}
