project2/grep-kmp/grep.dfy
@@ -6,9 +6,84 @@
  */
 
 include "Io.dfy"
+include "FileUtils.dfy"
+include "kmp.dfy"
+
+method Grep(file: FileStream, length: int32, pattern: seq<byte>) returns (ok:bool, found: bool, s:nat)
+  requires FileOk(file)
+  requires length as int == len(file)
+
+  modifies file
+  modifies file.env.ok
+  modifies file.env.files
+
+  ensures ok ==> FileOk(file)
+  ensures ok ==> found ==> 0 <= s < |content(file)|
+  ensures ok ==> !found ==> 0 <= s <= |content(file)|
+  ensures ok ==> found ==> match_at(content(file), pattern, s)
+  ensures ok ==> forall k :: 0 <= k < s ==> !match_at(content(file), pattern, k)
+{
+  var cont;
+  ok, cont := ReadFile(file, length as nat32);
+  if (!ok) {
+    return;
+  }
+
+  if (|cont| == 0) {
+    print "NO\n";
+    found := false;
+    s := 0;
+    return;
+  }
+
+  if (|pattern| == 0) {
+    print "YES\n";
+    found := true;
+    s := 0;
+    return;
+  }
+
+  found, s := Match(cont, pattern);
+}
 
 method {:main} Main(ghost env:HostEnvironment?)
   requires env != null && env.Valid() && env.ok.ok();
+  modifies env.ok
+  modifies env.files
 {
-  print "TODO!\n";  
+  var num_args := HostConstants.NumCommandLineArgs(env);
+
+  if (num_args != 3) {
+    print "Expected usage: grep <file>\n";
+    return;
+  }
+
+  var pattern := HostConstants.GetCommandLineArg(1, env);
+  var source := HostConstants.GetCommandLineArg(2, env);
+  var source_exists := FileStream.FileExists(source, env);
+
+  if (!source_exists) {
+    print ("Source file does not exist.\n");
+    return;
+  }
+
+  var ok1, src_file := FileStream.Open(source, env);
+  if (!ok1) {
+    print "Error while opening source file.\n";
+    return;
+  }
+
+  var ok2, src_len := FileStream.FileLength(source, env);
+  if (!ok2) {
+    print "Error while opening source file.\n";
+    return;
+  }
+
+  var ok, m, n := Grep(src_file, src_len, seqa2seqb(pattern[..]));
+}
+
+function method {:verify false} seqa2seqb(s: seq<char>): seq<byte>
+  decreases s
+{
+  if s == [] then [] else [s[0] as byte] + seqa2seqb(s[1..])
 }
